promise_free/examples/MPIA.v
@@ -1,10 +1,10 @@
 Require Import CRIS.
-Require Import PFMemHeader PFMemA base HistoryRA AtomicRA OneShotRA.
+Require Import PFMemHeader PFMemA base HistoryRA AtomicRA.
 Require Import SystemHeader SystemA SystemTactics.
 Require Import MPI MPA.
 
 Module MPIA. Section MPIA.
-  Context `{!crisG Γ Σ α β τ _S _I, !histG, !atomicG, !sysG, !one_shotG}.
+  Context `{!crisG Γ Σ α β τ _S _I, !concG, !histG, !atomicG, !sysG, !one_shotG}.
   Local Existing Instances one_shot_inG.
 
   Definition Ist : alist key Any.t → alist key Any.t → iProp Σ := λ _ _, emp%I.
@@ -21,29 +21,32 @@ Module MPIA. Section MPIA.
   Lemma mp2_spawnable : SystemA.fspec_spawnable sp_user MPHdr.mp2 MPA.mp2_precondition.
   Proof.
     exists MPA.mp2_spec; split; [eapply HMP; ss|].
-    intros [tid V]; ss; exists (tid, V); split.
-    { unfold_pre_post. iIntros (??) "[$ [% [-> [$ [% [-> P]]]]]]"; iModIntro; iFrame; ss. }
+    intros [tid stid]; ss; exists ((tid, stid)); split.
+    { unfold_pre_post. iIntros (??) "[$ [% [-> [% [$ [% [-> P]]]]]]]"; iModIntro; iFrame; ss. }
     { unfold_pre_post; iIntros (??) "[$ $] //". }
   Qed.
 
   Lemma simF_mp : ISim.sim_fun open MA MI MPA.init_cond%I IstFull None.
   Proof.
     init_simF.
-    iDestruct "IST" as "[[-> ->] TV]".
-    steps_l. iDestruct "ASM" as "[-> ->]". hss_l. steps_l.
+    (* iDestruct "IST" as "[[-> ->] TV]". *)
+    steps_l. iDestruct "ASM" as "->". hss_l. steps_l.
     steps_r. hss_r. steps_r.
+
     iApply wsim_system_yield; ss.
     { unfold_sp_exact sp_s SystemHdr.yield; ss. }
-    iFrame "TV". iSplit.
-    { iExists _, _, _, _; iSplit; eauto.
+    iFrame "TID". iSplit.
+    { iExists [], [], _, _; iSplit; eauto.
       iSplit; eauto.
       iSplit; eauto.
       iPureIntro; split; unfold_mod; prove_scope.
     }
+    iFrame.
     iIntros (??) "IST TV".
+    Unshelve. all: try exact ⊤.
 
     (* alloc *)
-    steps_r. inline_r. force_r (1%positive, 2, _). forces_r. iFrame. iSplit; eauto.
+    steps_r. inline_r. force_r (1%positive, 0, 2, _). forces_r. iFrame. iSplit; eauto.
     steps_r. iDestruct "GRT" as "[[%loc [%V' [[-> %LE] [TV [FA ↦]]]]] ->]".
     rewrite own_loc_na_vec_cons own_loc_na_vec_singleton.
     hss_r. steps_r.
@@ -54,6 +57,7 @@ Module MPIA. Section MPIA.
     iFrame "TV IST".
     clear dependent st_src st_tgt.
     iIntros (??) "IST TV".
+    Unshelve. all: try exact ⊤.
 
     (* yield *)
     steps_r.
@@ -62,10 +66,11 @@ Module MPIA. Section MPIA.
     iFrame "TV IST".
     clear dependent st_src st_tgt.
     iIntros (??) "IST TV".
+    Unshelve. all: try exact ⊤.
 
     (* write *)
     steps_r. inline_r.
-    force_r (existT 0 (1%positive, loc, Val.Vnum 0, Ordering.na, _)). forces_r.
+    force_r (existT 0 (1%positive, 0, loc, Val.Vnum 0, Ordering.na, _)). forces_r.
     rewrite shift_0.
     iFrame "TV".
     iDestruct "↦" as "[↦flag ↦data]"; iSplitL "↦flag".
@@ -81,10 +86,11 @@ Module MPIA. Section MPIA.
     iFrame "TV IST".
     clear dependent st_src st_tgt.
     iIntros (??) "IST TV".
+    Unshelve. all: try exact ⊤.
 
     (* write *)
     steps_r. inline_r.
-    force_r (existT 0 (1%positive, loc >> 1, Val.Vnum 0, Ordering.na, _)). forces_r.
+    force_r (existT 0 (1%positive, 0, loc >> 1, Val.Vnum 0, Ordering.na, _)). forces_r.
     iPoseProof (own_loc_na_own_loc with "↦data") as "$".
     iFrame "TV".
     iSplit; eauto.
@@ -98,19 +104,20 @@ Module MPIA. Section MPIA.
     iFrame "TV IST".
     clear dependent st_src st_tgt.
     iIntros (??) "IST TV".
+    Unshelve. all: try exact ⊤.
 
     (* spawn *)
     iMod (own_alloc Pending) as "[%γ O]"; ss.
     iMod (AtomicPtsTo_from_na loc (Val.Vnum 0) with "↦flag")
       as "[%γx [% [% [% [% [% [% [SW ↦flag]]]]]]]]".
-    iMod (inv_alloc_simple (MPA.mp_inv' 0 loc (loc >> 1) γ γx) _ _ MPA.mpN with "[↦flag]") as "#I".
-    { set_solver. }
+    iMod (inv_alloc (MPA.mp_inv' 0 loc (loc >> 1) γ γx) 1 _ _ MPA.mpN with "[↦flag]") as "#I"; eauto.
     { rewrite MPA.mp_inv'_eq.
       SL_red; iExists _; SL_red; iExists false.
       do 6 (SL_red; iExists _).
       SL_red; iSplit; last done.
       rewrite syn_AtomicPtsTo_red; iFrame.
     }
+    iPoseProof (AtomicSWriter_AtomicSeen with "SW") as "#SN".
 
     (* source yield *)
     iApply wsim_system_yield_src.
@@ -118,13 +125,14 @@ Module MPIA. Section MPIA.
     (* iApply wsim_system_yield_src. steps_l. *)
 
     (* spawn *)
-    force_l (1%positive, MPA.mp2_precondition, V3). forces_l.
+    force_l (1%positive, 0, MPA.mp2_precondition, V3). forces_l.
     iFrame "TV".
-    iSplitL "↦data".
+    iSplitL "↦data SW".
     { iExists _; iSplit; first done.
       iExists _, _, _; iSplit; first (iPureIntro; esplits; eauto using mp2_spawnable).
-      rewrite /MPA.mp2_precondition /MPA.mp_inv; iFrame "↦data".
-      rewrite shift_0; iExists _, _; iSplit; eauto.
+      rewrite /MPA.mp2_precondition /MPA.mp_inv; iFrame "↦data SW".
+      iExists γ; iSplit; eauto.
+      rewrite shift_0; eauto.
     }
     steps_l. steps_r. call "IST".
 
@@ -135,13 +143,13 @@ Module MPIA. Section MPIA.
     (* iRevert "I FA O SW IST TV". *)
     iStopProof.
 
-    revert st_s'. combine_quant st_t'. clear Hle3 H3. combine_quant V3.
+    revert st_s'. combine_quant st_t'. clear Hle3 H4. combine_quant V3.
     eapply wsim_coind.
     (* destruct_quant. *)
-    iIntros (g' [V3 [st_t st_s]]) "[#I [FA [P [SW [IST TV]]]]] _ #CIH"; s.
+    iIntros (g' _ CIH [V3 [st_t st_s]]) "[#[I SN] [FA [P [IST TV]]]]"; s.
 
-    unfold_iter_l. steps_l.
-    unfold_iter_r.
+    unfold_iterC_l. steps_l.
+    unfold_iterC_r.
 
     (* yield *)
     steps_r.
@@ -150,6 +158,7 @@ Module MPIA. Section MPIA.
     iFrame "TV IST".
     clear dependent st_s st_t.
     iIntros (??) "IST TV".
+    Unshelve. all: try exact ⊤.
 
     steps_r. inline_r.
     iInv "I" as "INV" "ACC".
@@ -159,14 +168,13 @@ Module MPIA. Section MPIA.
     { (* read 0 from flag *)
       iEval (SL_red; rewrite syn_AtomicPtsTo_red) in "INV"; iDestruct "INV" as "[↦flag ->]".
       rewrite AtomicPtsTo_eq. iDestruct "↦flag" as "[% ↦flag]".
-      force_r (existT 1 (1%positive, loc, Ordering.acqrel, _, _, _, _, _, _, _, _)). forces_r.
-      iPoseProof (AtomicSWriter_AtomicSeen with "SW") as "#SN".
+      force_r (existT 1 (1%positive, 0, loc, Ordering.acqrel, _, _, _, _, _, _, _, _)). forces_r.
       iFrame "TV SN ↦flag". iSplit; eauto.
       steps_r.
       iDestruct "GRT" as "[[% [% [% [% [% [% [%V4 [[-> %] [#SN2 [↦flag TV]]]]]]]]]] ->]".
       hss_r. steps_r.
       iMod ("ACC" with "[↦flag]") as "_".
-      { rewrite {3}MPA.mp_inv'_eq; SL_red; iExists _.
+      { rewrite {2}MPA.mp_inv'_eq; SL_red; iExists _.
         SL_red; iExists false.
         do 6 (SL_red; iExists _); SL_red.
         rewrite syn_AtomicPtsTo_red AtomicPtsTo_eq /AtomicPtsTo_def; iFrame.
@@ -181,10 +189,10 @@ Module MPIA. Section MPIA.
       iIntros (??) "IST TV".
 
       steps_r.
-      hexploit (H5 (Cell.max_ts ζ'')); first done; rewrite Cell.singleton_get.
+      hexploit (H6 (Cell.max_ts ζ'')); first done; rewrite Cell.singleton_get.
       des_if; intros INV; inv INV.
       destruct v'; ss.
-      apply Z.eqb_eq in H3; subst.
+      apply Z.eqb_eq in H4; subst.
       steps_r.
 
       steps_r.
@@ -199,9 +207,10 @@ Module MPIA. Section MPIA.
       iApply wsim_progress.
       iApply wsim_base.
       iIntros "W".
-      iSpecialize ("CIH" $! (V4, (st_tgt, st_src))); s.
-      iApply ("CIH" with "[-]"); iFrame. iFrame "I".
-      iEval (rewrite H7) in "SW"; iFrame.
+
+      iApply ((CIH (V4, (st_tgt, st_src))) with "[-]"); iFrame. iFrame "I".
+      ss. iModIntro. iEval (rewrite H8) in "SN". done.
+      Unshelve. all: try exact ⊤; try exact 1%Qp.
     }
     { (* read 1 from flag *)
       iDestruct "INV" as "[↦flag INV]".
@@ -211,8 +220,8 @@ Module MPIA. Section MPIA.
       rewrite syn_AtomicPtsTo_red.
       iEval (rewrite AtomicPtsTo_eq /AtomicPtsTo_def /view_at) in "↦flag".
       iDestruct "↦flag" as "[% ↦flag]".
-      force_r (existT 1 (_, _, _, _, _, _, _, _, _, V3, x2)). forces_r.
-      iPoseProof (AtomicSWriter_AtomicSeen with "SW") as "#SN".
+      force_r (existT 1 (_, _, _, _, _, _, _, _, _, _, V3, x2)). forces_r.
+      (* iPoseProof (AtomicSWriter_AtomicSeen with "SW") as "#SN". *)
       iFrame "TV SN ↦flag". iSplit; eauto.
       steps_r.
       iDestruct "GRT" as "[[% [% [% [% [% [% [% [[-> %Hres] [#SN2 [↦flag TV]]]]]]]]]] ->]".
@@ -221,7 +230,7 @@ Module MPIA. Section MPIA.
       erewrite Cell.add_o; eauto; des_if.
       { (* read 1 *)
         subst. intros INV; inv INV.
-        iClear "CIH".
+        (* iClear "CIH". *)
         destruct v'; ss. apply Z.eqb_eq in Hval; subst.
         hss_r; steps_r.
         iMod ("ACC" with "[↦flag P]") as "_".
@@ -247,6 +256,7 @@ Module MPIA. Section MPIA.
         clear dependent st_src st_tgt.
         iIntros (??) "IST TV".
         steps_r.
+        Unshelve. all: try exact ⊤.
 
         (* yield *)
         iApply wsim_system_yield; ss.
@@ -257,7 +267,7 @@ Module MPIA. Section MPIA.
         steps_r.
 
         (* non-atomic load here *)
-        inline_r. force_r (existT 0 (_, _, _, _, _, _)). forces_r.
+        inline_r. force_r (existT 0 (_, _, _, _, _, _, _)). forces_r.
         iEval (rewrite syn_own_loc_na_red) in "INV".
         assert (Hawk : Ordering.le Ordering.acqrel Ordering.acqrel) by refl.
         rewrite Hvle2 Hawk Hvle.
@@ -272,6 +282,7 @@ Module MPIA. Section MPIA.
         clear dependent st_src st_tgt.
         iIntros (??) "IST TV".
         steps_r.
+        Unshelve. all: try exact ⊤.
 
         destruct v'; ss. eapply Z.eqb_eq in Hval'; subst.
         steps_r.
@@ -280,6 +291,7 @@ Module MPIA. Section MPIA.
         forces_l. iSplit; eauto.
         step.
         iSplit; eauto.
+        Unshelve. all: try exact ⊤; try exact 1%Qp.
       }
       { (* read 0 *)
         rewrite Cell.singleton_get; des_if; intros INV; inv INV.
@@ -315,22 +327,23 @@ Module MPIA. Section MPIA.
         iApply wsim_progress.
         iApply wsim_base.
         iIntros "W".
-        iSpecialize ("CIH" $! (_, (st_tgt, st_src))); s.
+        (* iSpecialize ("CIH" $! ); s. *)
 
-        iApply ("CIH" with "[-]"); iFrame. iFrame "I".
-        iEval (rewrite Hvle) in "SW"; iFrame.
+        iApply ((CIH (_, (st_tgt, st_src))) with "[-]"); iFrame. iFrame "I".
+        iEval (rewrite Hvle) in "SN"; s; iModIntro; done.
       }
     }
-  Unshelve. all: try exact ∅. all: try exact 1%Qp.
+  Unshelve. all: try exact 1%Qp; try exact ⊤.
   (*SLOW*)Admitted.
 
   Lemma simF_mp2 : ISim.sim_fun open MA MI MPA.init_cond%I IstFull (Some MPHdr.mp2).
   Proof.
     init_simF.
     steps_l.
-    iDestruct "ASM" as "[%va [-> [%sa [-> [PRE TV]]]]]".
-    rename _q1 into tid, _q2 into V. hss_l.
-    rewrite /MPA.mp2_precondition; iDestruct "PRE" as "[%loc [%γ [%γx [[-> ->] [#I ↦data]]]]]".
+    iDestruct "ASM" as "[%va [-> [%sa [%V [-> [PRE TV]]]]]]".
+    rename _q1 into tid, _q2 into stid. hss_l.
+    rewrite /MPA.mp2_precondition.
+    iDestruct "PRE" as "[%loc [%γ [%γx [%V0 [%fd [%td [% [% [[-> ->] [#I [↦data ⊒]]]]]]]]]]]".
     steps_l. hss_l. steps_l.
 
     rewrite /MPA.mp2. steps_l.
@@ -345,6 +358,7 @@ Module MPIA. Section MPIA.
     clear dependent st_src st_tgt.
     iIntros (??) "IST TV".
     steps_r.
+    Unshelve. all: try exact ⊤.
 
     (* yield *)
     iApply wsim_system_yield; ss.
@@ -353,10 +367,11 @@ Module MPIA. Section MPIA.
     clear dependent st_src st_tgt.
     iIntros (??) "IST TV".
     steps_r.
+    Unshelve. all: try exact ⊤.
 
     (* write to data *)
     inline_r.
-    force_r (existT 0 (_, _, _, _, _)). forces_r.
+    force_r (existT 0 (_, _, _, _, _, _)). forces_r.
     iPoseProof (own_loc_na_own_loc with "↦data") as "↦data".
     iFrame "TV ↦data". iSplit; eauto.
     steps_r. iDestruct "GRT" as "[[%V2 [[-> %Hle] [↦data TV]]] ->]".
@@ -369,7 +384,79 @@ Module MPIA. Section MPIA.
     clear dependent st_src st_tgt.
     iIntros (??) "IST TV".
     steps_r.
+    Unshelve. all: try exact ⊤.
 
     (* open invariant *)
-  Admitted.
-End MPIA. End MPIA.
+    (* iMod (AtomicPtsToX_from_na _  _ V2 with "↦data") as "[%γd [%f [%t [%Hft [%V0 [% [%H02 [sw swX]]]]]]]]". *)
+    iInv "I" as "INV" "ACC".
+    iEval (rewrite MPA.mp_inv'_eq /MPA.mp_inv'_def; SL_red) in "INV".
+    do 8 (iDestruct "INV" as "[% INV]"; iEval (SL_red) in "INV").
+    iDestruct "INV" as "[↦flag _]".
+    rewrite syn_AtomicPtsTo_red.
+    rewrite shift_0; iPoseProof (AtomicPtsTo_SWriter_agree with "[$] [$]") as "->".
+
+    inline_r. steps_r.
+    iEval (rewrite AtomicPtsTo_eq /AtomicPtsTo_def /view_at) in "↦flag".
+    iDestruct "↦flag" as "[% ↦flag]".
+    force_r (existT 1 (tid, stid, loc, Val.Vnum 1, Ordering.acqrel, V2, γx, _, _, _, _, _, _, _)).
+    forces_r.
+    iFrame "↦flag". iSplitL "⊒ TV"; eauto.
+    { iSplit; eauto. iSplit; eauto. iFrame. tview_sync Hle.
+      iPoseProof (AtomicSWriter_AtomicSeen with "⊒") as "#sn"; iSplit; eauto.
+      rewrite AtomicSWriter_eq /AtomicSWriter_def /view_at /=; iDestruct "⊒" as "[? [? ?]]"; iFrame.
+    }
+    Unshelve. all: try exact 1%Qp.
+    steps_r.
+
+    iDestruct "GRT" as "[[% [% [% [% [% [% [[-> [%Htime %Hres]] [sn [at [sy [swX tv]]]]]]]]]]] ->]".
+    destruct (Ordering.le _ _) eqn : Heqb in Hres; ss; subst; clear Heqb.
+    rewrite Cell.max_ts_singleton in Htime.
+    hss_r. steps_r.
+    iMod ("ACC" with "[↦data swX]") as "_".
+    { rewrite MPA.mp_inv'_eq.
+      SL_red; iExists _; SL_red; iExists true.
+      do 6 (SL_red; iExists _).
+      SL_red.
+      rewrite syn_AtomicPtsTo_red; iFrame.
+      iSplitL "swX".
+      { rewrite AtomicPtsTo_eq /AtomicPtsTo_def /view_at; iExists t; iFrame. }
+      do 3 (SL_red; iExists _); SL_red.
+      iSplitR "↦data".
+      iPureIntro. split; cycle 1; eauto.
+      iRight; rewrite syn_own_loc_na_red.
+      iApply (own_loc_mon_pred_gen with "↦data"); eauto; try exact 1%Qp.
+      apply View.join_l.
+    }
+
+    iApply wsim_system_yield; ss.
+    { unfold_sp_exact sp_s SystemHdr.yield; ss. }
+    iFrame "tv IST". clear dependent st_src st_tgt; iIntros (st_src st_tgt) "IST TID".
+    steps_r.
+
+    iApply (wsim_system_yield_src with "[-]"). steps_l. forces_l.
+    iFrame. iSplitR; [eauto|]. step. iFrame. done. 
+  Unshelve. all: try exact ⊤.
+  Qed.
+
+  Lemma sim : ISim.t open MA MI MPA.init_cond IstFull.
+  Proof.
+    init_sim.
+    { eapply simF_mp2. }
+    { eapply simF_mp. }
+  Qed.
+End MPIA.
+Section ctxr.
+  Context `{!crisG Γ Σ α β τ _S _I, !concG, !histG, !atomicG, !sysG, !one_shotG}.
+
+  Definition ctxr (sp_s : sp_type) (sp_user : spl_type) :
+    sp_incl (SystemA.sp sp_user ⊤) sp_s →
+    spl_sub MPA.sp sp_user →
+    ctx_refines
+      ((MPA.t sp_s ★ SystemA.t sp_user sp_s ★ PFMemA.t sp_s), MPA.init_cond)
+      ((MPI.t      ★ SystemA.t sp_user sp_s ★ PFMemA.t sp_s), True%I).
+  Proof using.
+    intros ??.
+    eapply main_adequacy, sim; eauto.
+  Qed.
+End ctxr.
+End MPIA.
