promise_free/examples/MPAll.v
@@ -1,0 +1,178 @@
+(* Require Import CRIS Cancel.
+Require Import PFMemHeader PFMemA base HistoryRA AtomicRA PFMemA PFMemI PFMemIAproof.
+Require Import SystemHeader SystemI SystemA SystemIA SystemTactics.
+Require Import MPI MPA MPIA.
+Require Import Language.
+
+Module MPAll.
+  Import inv_instances.
+
+  Definition lang := Language.mk (λ _ : (), tt) (const False) (λ _ : ProgramEvent.t, λ _ _, True).
+  Definition syn : Threads.syntax := IdentMap.singleton 1%positive (existT lang tt).
+  Definition init : Configuration.t := Configuration.init syn [].
+
+  Local Instance Γ : HRA := ##[invΓ; concΓ; memΓ; newSystemΓ; incrΓ].
+  Local Instance Σ : GRA := ##[Γ; invΣ; newschΣ].
+
+  Definition irΓ : Γ :=
+    **[ir_invΓ; ir_concΓ; ir_memΓ csl genv; SchA.ir_schΓ; *[None]].
+  Definition irΣ : Σ :=
+    **[irΓ; ir_invΣ; SchA.ir_schΣ].
+
+  Lemma irΣ_valid : ✓ (irΣ ⋅ ir_own_admin).
+  Proof.
+    solve_ir_valid.
+    - apply ir_tidRA_valid.
+    - apply ir_yieldRA_valid.
+    - apply ir_memRA_valid.
+    - apply SchA.ir_newtidRA_valid.
+    - apply SchA.ir_joinRA_valid.
+  Qed.
+
+  (* source module *)
+  Local Definition sp_user_s : spl_type := ClientA.sp ⊤.
+  Local Definition smod_src : SMod.t := (ClientA.smod ⊤) ☆ (SchA.smod sp_user_s).
+  Local Definition mod_top : Mod.t := SMod.to_mod sp_none (SMod.cancel smod_src).
+  Local Definition mod_tgt : Mod.t := ClientI.t ★ FaaI.t ★ (MemI.t csl genv) ★ (SchI.t).
+
+  Local Definition sp : string → option fspec := sp_from smod_src.
+  Local Definition mod_src : Mod.t := SMod.to_mod sp smod_src.
+
+  (* Local Definition SchInSp0: sp_incl (SchAS.sp ⊤ (to_sp [])) (to_sp (SchAS.sp ⊤ (to_sp []))).
+  Proof.
+    split; [|refl]. rewrite /SchAS.sp; unseal CRIS. prove_nodup.
+  Qed. *)
+  Local Definition SchInSp : sp_incl (SchA.sp sp_user_s ⊤) sp.
+  Proof.
+    rewrite /SchA.sp; unseal CRIS.
+    split; [prove_nodup|].
+    intros ??; ss; des_ifs; des_sumbool; clarify; intros INV; inv INV;
+      rewrite /sp /smod_src /sp_from /= /to_sp /=; des_ifs; ss.
+  Qed.
+  Local Definition UserInSp : sp_incl sp_user_s sp.
+  Proof.
+    rewrite /sp_user_s /ClientA.sp /MemA.sp; unseal CRIS.
+    split; [prove_nodup|].
+    intros ??; ss; des_ifs; des_sumbool; clarify; intros INV; inv INV;
+      rewrite /sp /smod_src /sp_from /= /to_sp /=; des_ifs; ss.
+  Qed.
+  Local Definition MainInSp : spl_sub (ClientA.sp ⊤) sp_user_s.
+  Proof.
+    rewrite /spl_sub /sp_user_s /ClientA.sp /ClientA.incr_spec /=.
+    ii; rewrite ->eq_rel_dec_correct in *; des_ifs.
+  Qed.
+  (* Local Definition MemInSp : sp_incl MemA.sp sp.
+  Proof.
+    ii; rewrite /sp /SchAS.sp /MemA.sp /ClientA.sp; unseal CRIS; split; [prove_nodup|ii].
+    ss; des_ifs; rewrite ->eq_rel_dec_correct in *; des_ifs.
+  Qed. *)
+
+  Local Definition init_cond : iProp Σ :=
+    MemA.init_cond csl genv ∗ SchA.init_cond ∗ ClientIA.ClientIA.init_cond ⊤.
+  (* Local Definition main_fsp : fspec := ClientA.main_spec ⊤ 1%Qp. *)
+
+  (* Apply cancellation to linked spec module *)
+  Lemma cancel_src :
+    refines (mod_top, init_cond ∗ TIDAUTH 0 ∗ YIELDAUTH 1)%I (mod_src, init_cond).
+  Proof.
+    eapply Cancel.cancellation.
+    { ii; des; subst; inv FIND; ss.
+      rewrite !eq_rel_dec_correct in H0; des_ifs.
+    }
+  Qed.
+
+  (* Refinement between spec/impl of whole program (linked module) *)
+  Lemma src_tgt : refines (mod_src, init_cond) (mod_tgt, emp%I).
+  Proof.
+    eapply ctxr_refines.
+    rewrite /mod_src /mod_tgt /smod_src !add_interp_comm.
+
+    (* abstraction of Sch *)
+    etrans; cycle 1.
+    { do 3 ctxr_drop.
+      eapply main_adequacy, SchIA.sim.
+      - apply SchInSp.
+      - apply UserInSp.
+    }
+
+    (* abstraction of Mem *)
+    etrans; cycle 1.
+    { do 3 ctxr_rotate. do 3 ctxr_drop.
+      eapply MemIA.ctxr.
+    }
+
+    (* abstraction of Faa *)
+    etrans; cycle 1.
+    { do 2 ctxr_drop.
+      eapply main_adequacy, FaaIA.sim.
+    }
+    rewrite /FaaIA.FaaIA.MA.
+    
+    (* abstraction of Incr *)
+    etrans; cycle 1.
+    { ctxr_drop.
+      eapply ClientIA.ctxr.
+      - instantiate (1:=⊤). set_solver.
+      - apply MainInSp.
+      - apply SchInSp.
+    }
+
+    etrans; cycle 1.
+    { ctxr_rotate. ctxr_refl. }
+
+    (* elimination of mem *)
+    etrans; cycle 1.
+    { do 2 ctxr_rotate. do 2 ctxr_drop. eapply CFilter.elim_module. }
+    rewrite -mod_add_empty_r.
+
+    rewrite /SchIAproof.SchIA.SchAMod.
+    rewrite /SchA.t /ClientA.t /MemA.t.
+    unseal CRIS.
+    ctxr_rotate.
+    
+    eapply ctxr_cond_strengthen.
+    { iIntros "[? [? ?]]". iFrame. }
+  (*SLOW*)Qed.
+
+  Lemma top_tgt :
+    refines (mod_top, init_cond ∗ TIDAUTH 0 ∗ YIELDAUTH 1)%I
+            (mod_tgt, emp%I).
+  Proof.
+    etrans.
+    { eapply cancel_src. }
+    { eapply src_tgt. }
+  Qed.
+
+  Lemma tgt_wf:
+    Mod.wf mod_tgt.
+  Proof.
+    rewrite /mod_tgt /ClientI.t /FaaI.t /MemI.t /SchI.t; unseal CRIS; prove_nodup.
+  Qed.
+
+  Lemma init_cond_valid:
+    ∃ rs, ✓ rs ∧ (Own rs ⊢ |==> init_cond ∗ TIDAUTH 0 ∗ YIELDAUTH 1).
+  Proof.
+    exists (irΣ ⋅ ir_own_admin). split.
+    - apply irΣ_valid.
+    - simplify_res.
+      { rewrite make_own_admin.
+        iDestruct "H24" as "[H24 Htid]". iFrame.
+        rewrite /MemA.init_cond /ir_memRA; iDestruct "H26" as "[$ _]".
+        iPoseProof (make_sys_init with "[$] [$]") as "[$ [$ [$ $]]]". done.
+      }
+    all: solve_res.
+  Qed.
+
+  Theorem behavioral_refinement :
+    ∃ src_res tgt_res, refines_lmod
+      (Mod.to_lmod mod_top src_res)
+      (Mod.to_lmod mod_tgt tgt_res).
+  Proof.
+    move: (top_tgt)=>H; rewrite /refines in H; des; ss.
+    hexploit H; eauto using tgt_wf. clear H; intros [WF H].
+    assert (IV:= init_cond_valid). des.
+    destruct (H rs); des; et.
+    rewrite IV0 /init_cond /ClientIA.ClientIA.init_cond /ClientA.init_cond.
+    rewrite {1}winv_split_empty. iIntros ">[[$ [$ [[$ $] $]]] $]". done.
+  (*SLOW*)Qed.
+End MPAll. *)
