promise_free/system/SystemTactics.v
@@ -1,14 +1,12 @@
 Require Import CRIS SystemHeader SystemA.
 
-Require Import ltac2_lib.
-
 Section wsim.
   Context `{!crisG Γ Σ α β τ _S _I, !concG, !sysG}.
 
-  (* Lemma wsim_system_yield
+  Lemma wsim_system_yield
       fl_src fl_tgt Ist r g R_src R_tgt RR p_src p_tgt
       st_src st_tgt itr_src itr_tgt
-      (tid : Ident.t) (V : TView.t)
+      (tid : Ident.t) (stid : nat) (V : TView.t)
       (E E_src E_tgt : coPset)
       (img_src img_tgt : bool)
       (msk_src msk_tgt : string → bool)
@@ -22,95 +20,81 @@ Section wsim.
     (sp_src SystemHdr.yield = if img_src then Some (SystemA.yield_spec E_src) else None) →
     (sp_tgt SystemHdr.yield = if img_tgt then Some (SystemA.yield_spec E_tgt) else None) →
     Ist st_src st_tgt ∗
-    (if ((negb img_tgt) && img_src) then tview_sys tid V else emp) ∗
+    (if ((negb img_tgt) && img_src) then tview_sys tid stid V else emp) ∗
     (∀ st_src st_tgt,
       Ist st_src st_tgt -∗
-      (if ((negb img_tgt) && img_src) then tview_sys tid V else emp) -∗
-      wsim fl_src fl_tgt Ist (E, E) r g R_src R_tgt RR p_src true
-        (st_src, SB.sandbox img_src msk_src scp_src (SModTr.trans sp_src 𝒴) >>= itr_src)
+      (if ((negb img_tgt) && img_src) then tview_sys tid stid V else emp) -∗
+      wsim fl_src fl_tgt Ist (E, E) r g R_src R_tgt RR true true
+        (st_src, SB.sandbox img_src msk_src scp_src (SModTr.trans true sp_src 𝒴) >>= itr_src)
         (st_tgt, itr_tgt ())) ⊢
     wsim fl_src fl_tgt Ist (E, E) r g R_src R_tgt RR p_src p_tgt
-      (st_src, SB.sandbox img_src msk_src scp_src (SModTr.trans sp_src 𝒴) >>= itr_src)
-      (st_tgt, SB.sandbox img_tgt msk_tgt scp_tgt (SModTr.trans sp_tgt 𝒴) >>= itr_tgt).
+      (st_src, SB.sandbox img_src msk_src scp_src (SModTr.trans true sp_src 𝒴) >>= itr_src)
+      (st_tgt, SB.sandbox img_tgt msk_tgt scp_tgt (SModTr.trans false sp_tgt 𝒴) >>= itr_tgt).
   Proof.
     intros -> ? Himg ?? Hsrc Htgt.
     rewrite /System.yield; unseal "System".
     revert p_src. combine_quant p_tgt.
     combine_quant st_src. combine_quant st_tgt.
     eapply wsim_coind.
-    iIntros (g' [st_src [st_tgt [p_tgt p_src]]]) "[IST [TV KTR]] %LE /= #CIH".
+    iIntros (g' Hgg' CIH [st_tgt [st_src [p_src p_tgt]]]) "[IST [TV KTR]] /=".
+    destruct_quant CIH.
 
-    unfold_iter_r.
-    steps_r. destruct _q.
+    unfold_iterC_r.
+    steps_r. destruct _q as [[|]|]; cycle 2.
     { steps_r.
+      unfold_iterC_l. steps_l. force_l (Some false). steps_l.
       iApply wsim_unfold; iIntros "W".
       iApply wsim_mono_knowledge; cycle 2.
       { iApply wsim_fold; iFrame "W". iApply ("KTR" with "IST TV"). }
       { ii; iIntros "$ !> //". }
-      { ii; iIntros "G"; iPoseProof (LE with "G") as "$"; done. }
+      { ii; iIntros "G"; iPoseProof (Hgg' with "G") as "$"; done. }
     }
+    { destruct img_tgt; cycle 1.
+      { steps_r. rewrite Htgt /=.
+        unfold_iterC_l. steps_l.
+        iApply wsim_progress.
+        force_l (Some true). steps_l.
+        destruct img_src; cycle 1.
+        { rewrite Hsrc /=. steps_l. steps_r.
+          call "IST".
+          steps_l. hss. steps_l.
+          steps_r. hss_r. step_r.
+          by_coind CIH.
+          iFrame.
+        }
+        { rewrite Hsrc /=.
+          force_l (tid, stid, V). steps_l. forces_l.
+          iFrame "TV". iSplit; eauto.
+          steps_l. steps_r.
+          call "IST".
+          steps_l. iDestruct "ASM" as "[[-> TV] ->]". hss.
+          steps_l. steps_r. hss_r. steps_r.
+          by_coind CIH.
+          iFrame.
+        }
+      }
 
-    destruct img_tgt; cycle 1.
-    { steps_r. rewrite Htgt /=.
-      unfold_iter_l. steps_l.
-      iApply wsim_progress.
-      force_l false. steps_l.
       destruct img_src; cycle 1.
-      { rewrite Hsrc /=. steps_l. steps_r.
-        call "IST".
-        steps_l. hss. steps_l.
-        steps_r. hss_r. step_r.
-        iApply wsim_base.
-        iSpecialize ("CIH" $! _);
-          (hrepeat do 1 first[instantiate (1:= (_,_))|instantiate (1:= existT _ _)]); s; grind.
-        iIntros "W"; iApply "CIH".
-        iFrame. iIntros (??) "I _"; iPoseProof ("KTR" with "I") as "KTR".
-        iApply (wsim_flag_mon with "[KTR]"); cycle 2.
-        { iApply "KTR"; done. }
-        all: eauto.
-      }
-      { rewrite Hsrc /=.
-        force_l (tid, V). steps_l. forces_l.
-        iFrame "TV". iSplit; eauto.
-        steps_l. steps_r.
-        call "IST".
-        steps_l. iDestruct "ASM" as "[[-> TV] ->]". hss.
-        steps_l. steps_r. hss_r. steps_r.
-        iApply wsim_base.
-        iSpecialize ("CIH" $! _);
-          (hrepeat do 1 first[instantiate (1:= (_,_))|instantiate (1:= existT _ _)]); s; grind.
-        iIntros "W"; iApply "CIH".
-        iFrame. iIntros (??) "I TV"; iPoseProof ("KTR" with "I") as "KTR".
-        iApply (wsim_flag_mon with "[-]"); cycle 2.
-        { iApply "KTR"; done. }
-        all: eauto.
-      }
+      { hexploit Himg; ss. }
+      steps_r. rewrite Htgt /=. steps_r.
+      iClear "TV"; iDestruct "GRT" as "[[-> TV] _]".
+
+      unfold_iterC_l. steps_l. force_l (Some true). steps_l.
+      rewrite Hsrc /=. force_l (_, _, _). steps_l.
+      rewrite difference_union_L (comm_L union) subseteq_union_1_L //.
+
+      forces_l. iFrame "TV". iSplit; eauto.
+      steps_l. call "IST".
+      steps_l. iDestruct "ASM" as "[[-> TV] ->]". hss.
+      steps_l. forces_r. iFrame "TV"; iSplit; eauto.
+      steps_r.
+      hss_r. steps_r.
+      by_coind CIH.
+      iFrame.
     }
-
-    destruct img_src; cycle 1.
-    { hexploit Himg; ss. }
-    steps_r. rewrite Htgt /=. steps_r.
-    iClear "TV"; iDestruct "GRT" as "[[-> TV] _]".
-
-    unfold_iter_l. steps_l. force_l false. steps_l.
-    iApply wsim_progress.
-    rewrite Hsrc. force_l (_q1, _q2). steps_l.
-    rewrite difference_union_L (comm_L union) subseteq_union_1_L //.
-
-    forces_l. iFrame "TV". iSplit; eauto.
-    steps_l. call "IST".
-    steps_l. iDestruct "ASM" as "[[-> TV] ->]". hss.
-    steps_l. forces_r. iFrame "TV"; iSplit; eauto.
-    steps_r.
-    hss_r. steps_r.
-    iApply wsim_base.
-    iSpecialize ("CIH" $! _);
-      (hrepeat do 1 first[instantiate (1:= (_,_))|instantiate (1:= existT _ _)]); s; grind.
-    iIntros "W"; iApply "CIH".
-    iFrame. iSplit; first done. iIntros (??) "I TV"; iPoseProof ("KTR" with "I") as "KTR".
-    iApply (wsim_flag_mon with "[-]"); cycle 2.
-    { iApply "KTR"; done. }
-    all: eauto.
+    steps_r. unfold_iterC_l; steps_l; force_l (Some false); steps_l.
+    by_coind CIH.
+    iFrame.
   (*SLOW*)Qed.
 
   Lemma wsim_system_yield_src
@@ -124,11 +108,11 @@ Section wsim.
       (st_src, itr_src ())
       (st_tgt, itr_tgt) ⊢
     wsim fl_src fl_tgt Ist (E, E) r g R_src R_tgt RR p_src p_tgt
-      (st_src, SB.sandbox img_src msk_src scp_src (SModTr.trans sp_src 𝒴) >>= itr_src)
+      (st_src, SB.sandbox img_src msk_src scp_src (SModTr.trans img_src sp_src 𝒴) >>= itr_src)
       (st_tgt, itr_tgt).
   Proof.
     iIntros "S"; rewrite /System.yield; unseal "System".
-    unfold_iter_l; steps_l.
-    force_l true; steps_l; done.
-  Qed. *)
+    unfold_iterC_l; steps_l.
+    force_l (None); steps_l; done.
+  Qed.
 End wsim.
